src/Language/PlutusIR/Transform/Rename/SSP.v
@@ -1,0 +1,221 @@
+Require Import PlutusCert.Language.PlutusIR.
+Import NamedTerm.
+Require Import PlutusCert.Language.PlutusIR.Transform.Rename.
+Require Import PlutusCert.Language.PlutusIR.Analysis.FreeVars.
+
+Require Import Coq.Logic.FunctionalExtensionality.
+
+(*
+Require Import Coq.Lists.List.
+Import ListNotations.
+*)
+
+Require Import Coq.Strings.String.
+Local Open Scope string_scope.
+
+Require Import PlutusCert.Language.PlutusIR.Semantics.Static.
+Require Import PlutusCert.Language.PlutusIR.Semantics.Static.Implementations.Named.
+
+Definition rename_result := @rename_result name.
+Definition environment := list (name * rename_result).
+Definition lookupRR : environment -> name -> option rename_result := lookupRR eqb.
+Definition lookupV : environment -> rename_result -> option name := lookupV eqb.
+Definition Rename : environment -> Term -> Term -> Type := Rename eqb.
+Definition RenameBindingsNonRec : environment -> environment -> list Binding -> list Binding -> Type := RenameBindingsNonRec eqb.
+Definition RenameBindingsRec : environment -> environment -> list Binding -> list Binding -> Type := RenameBindingsRec eqb.
+Definition RenameBinding : environment -> environment -> Binding -> Binding -> Type := RenameBinding eqb.
+Definition Rename_dtdecl : environment -> environment -> DTDecl -> DTDecl -> Type := Rename_dtdecl eqb.
+Definition Rename_var_bind : environment -> name * rename_result -> name -> name -> Type := @Rename_var_bind name tyname eqb.
+Definition Rename_constrs : environment -> environment -> list constructor -> list constructor -> Type := Rename_constrs eqb.
+Definition Rename_constr : environment -> name * rename_result -> constructor -> constructor -> Type := Rename_constr eqb.
+
+
+Fixpoint RenameContext (env : environment) (Gamma : Context) : Context :=
+  match env with
+  | nil => Gamma
+  | (x, RenamedTo u) :: env' => 
+      match lookupT Gamma x with
+      | None => 
+          RenameContext env' Gamma
+      | Datatypes.Some T => 
+          u |T-> T ; RenameContext env' (deleteT x Gamma)
+      end
+  | (x, Unchanged) :: env' => 
+      RenameContext env' Gamma
+  end.
+
+Compute (
+  lookupT 
+  (RenameContext (("a", RenamedTo "b") :: ("a" , RenamedTo "c") :: nil) ("a" |T-> Ty_Var "B"; "a" |T-> Ty_Var "C"; emptyContext))
+  "c"
+).
+
+Definition non_capturing_environment (t : Term) (env : environment) : Prop :=
+  forall x rr, 
+    List.In x (free_vars eqb t) ->
+    lookupRR env x = Datatypes.Some rr /\ lookupV env rr = Datatypes.Some x.
+
+Lemma e : forall env t y r,
+    non_capturing_environment t ((y, r) :: env) ->
+    non_capturing_environment t env.
+Proof.
+  intros.
+  unfold non_capturing_environment.
+  intros.
+  unfold non_capturing_environment in H.
+  apply H with x rr in H0.
+  destruct H0.
+  inversion H0.
+  inversion H1.
+  destruct (x =? y) eqn:Hxy; destruct (rename_result_eqb eqb rr r) eqn:Hrrr.
+  - inversion H3. subst.
+    inversion H4. subst.
+Abort.
+
+(* Predicate for the [has_type] datatype *)
+Definition P_ht Gamma t1 T := 
+  forall env t2, 
+    (forall x y T', 
+      lookupRR env x = Datatypes.Some (RenamedTo y) ->
+      lookupT Gamma x = Datatypes.Some T' -> 
+      lookupT (RenameContext env Gamma) y = Datatypes.Some T'
+    ) ->
+    Rename env t1 t2 -> 
+    (RenameContext env Gamma) |-+ t2 : T.
+
+(* Predicate for the [constructor_well_formed] datatype *)
+Definition P_cwf Gamma c := Gamma |-ok_c c.
+
+(* Predicate for the [bindings_well_formed_nonrec] datatype *)
+Definition P_bwfnr Gamma bs1 :=
+    forall env env' bs2,
+      Gamma |-oks_nr bs1 ->
+      RenameBindingsNonRec env env' bs1 bs2 ->
+      Gamma |-oks_nr bs2.
+
+(* Predicate for the [bindings_well_formed_rec] datatype *)
+Definition P_bwfr Gamma bs1 :=
+  forall env env' bs2,
+    Gamma |-oks_nr bs1 ->
+    RenameBindingsRec env env' bs1 bs2 ->
+    Gamma |-oks_nr bs2.
+
+(* Predicate for the [binding_well_formed] datatype *)
+Definition P_bwf Gamma b1 := 
+  forall env env' b2,
+      Gamma |-ok b1 ->
+      RenameBinding env env' b1 b2 ->
+      Gamma |-ok b2.
+
+Axiom skip : forall P, P.
+
+
+Lemma e0e0 : forall env x w T Gamma t T0,
+    ~(List.In x (free_vars eqb t)) ->
+    (RenameContext ((x, RenamedTo w) :: env) (x |T-> T0; Gamma)) |-+ t : T ->
+    (w |T-> T0; RenameContext env Gamma) |-+ t : T.
+Proof.
+  induction env.
+  - intros.
+    simpl in H0.
+    rewrite update_eq in H0.
+    destruct (w =? x) eqn:Heqb.
+    + apply eqb_eq in Heqb as Heq.
+      subst.
+      rewrite deleteT_eq in H0.
+      simpl.
+      apply skip.
+    + apply eqb_neq in Heqb as Hneq.
+      apply skip.
+  - intros.
+Admitted.
+
+Theorem Rename__SSP : forall Gamma t1 T,
+    Gamma |-+ t1 : T ->
+    P_ht Gamma t1 T.
+Proof.
+  apply has_type__ind with 
+    (P := P_ht) 
+    (P0 := P_cwf) 
+    (P1 := P_bwfnr) 
+    (P2 := P_bwfr) 
+    (P3 := P_bwf).
+  - (* T_Let *)
+    intros Gamma bs t T Gamma' Heq Htyp_bs IH_bs Htyp_t IH_t.
+    unfold P_ht.
+    intros env t2 X.
+    subst.
+
+    apply skip.
+  - (* T_LetRec *)
+    apply skip.
+
+  - (* T_Var *)
+    intros Gamma x T Hlookup.
+    unfold P_ht. 
+    intros env t2 Hnce X.
+    
+    inversion X.
+    + (* RenameVar *)
+      subst.
+      apply T_Var.
+      eapply Hnce; eauto.
+    + (* RenameVarEq *)
+      subst.
+      apply T_Var.
+      eapply Hnce.
+      apply skip.
+      apply skip.
+
+  - (* T_TyAbs *)
+    apply skip.
+  - (* T_LamAbs *)
+    intros Gamma x T1 t0 T2 Htyp_t0 IH_t0 Hkind_T1. 
+    unfold P_ht. 
+    intros env t2 Hnce X.
+
+    inversion X.
+    + (* RenameLamAbsRename *) 
+      subst.
+      rename t' into t0'.
+      apply T_LamAbs.
+      * unfold P_ht in IH_t0.
+        eapply IH_t0 in X0; eauto.
+        apply skip. apply skip.
+      * apply skip.
+    + apply skip.
+         
+  - (* T_Apply *)
+    apply skip.
+  - (* T_Constant *)
+    apply skip.
+  - (* T_Builtin *)
+    apply skip.
+  - (* T_TyInst *)
+    apply skip.
+  - (* T_Error *)
+    apply skip.
+  - (* T_IWrap *)
+    apply skip.
+  - (* T_Unwrap *)
+    apply skip.
+
+  - (* W_Con *)
+    apply skip.
+
+  - (* W_NilB_NonRec *)
+    apply skip.
+  - (* W_ConsB_NonRec *)
+    apply skip.
+  - (* W_NilB_Rec *)
+    apply skip.
+  - (* W_ConsB_Rec*)
+    apply skip.
+           
+  - (* W_Term *)
+    apply skip.
+  - (* W_Type *)
+    apply skip.
+  - (* W_Data *)
+    apply skip.
+Qed. 
